$$\gamma_1 = -1, \gamma_2 = -2$$$$\sigma_1 = \left(-1\right)+\left(0\right)\jmath, \sigma_2 = \left(-1\right)+\left(0\right)\jmath$$$$G_{\mathcal S}(t) = \left(\begin{array}{cc} \frac{1}{4}-\frac{t\,{\mathrm{e}}^{-2\,t}}{2}-\frac{t^2\,{\mathrm{e}}^{-2\,t}}{2}-\frac{{\mathrm{e}}^{-2\,t}}{4} & \frac{t^2\,{\mathrm{e}}^{-2\,t}}{2}\\ \frac{t^2\,{\mathrm{e}}^{-2\,t}}{2} & \frac{t\,{\mathrm{e}}^{-2\,t}}{2}-\frac{{\mathrm{e}}^{-2\,t}}{4}-\frac{t^2\,{\mathrm{e}}^{-2\,t}}{2}+\frac{1}{4} \end{array}\right)$$